<?xml version="1.0"?>
<rdf:RDF xmlns="http://www.semanticweb.org/decentralized-context-aware-ontology/"
     xml:base="http://www.semanticweb.org/decentralized-context-aware-ontology/"
     xmlns:owl="http://www.w3.org/2002/07/owl#"
     xmlns:rdf="http://www.w3.org/1999/02/22-rdf-syntax-ns#"
     xmlns:ssn="http://www.w3.org/ns/ssn/"
     xmlns:xml="http://www.w3.org/XML/1998/namespace"
     xmlns:xsd="http://www.w3.org/2001/XMLSchema#"
     xmlns:rdfs="http://www.w3.org/2000/01/rdf-schema#"
     xmlns:skos="http://www.w3.org/2004/02/skos/core#"
     xmlns:sosa="http://www.w3.org/ns/sosa/"
     xmlns:swrl="http://www.w3.org/2003/11/swrl#"
     xmlns:vann="http://purl.org/vocab/vann/"
     xmlns:decas="http://www.semanticweb.org/decentralized-context-aware-ontology#"
     xmlns:swrla="http://swrl.stanford.edu/ontologies/3.3/swrla.owl#"
     xmlns:swrlb="http://www.w3.org/2003/11/swrlb#"
     xmlns:terms="http://purl.org/dc/terms/"
     xmlns:schema="http://schema.org/">
    <owl:Ontology rdf:about="http://www.semanticweb.org/decentralized-context-aware-ontology">
        <terms:created rdf:datatype="http://www.w3.org/2001/XMLSchema#date">2023-11-05</terms:created>
        <terms:description xml:lang="en">This ontology models the Decentralized Context-Aware System (DeCAS) entity relation. It provides a range of sensor and actuators classes that reflect a manufacturer&apos;s mode.

This ontology is based on the SSN/SOSA IoT sensor network ontologies.</terms:description>
        <terms:title xml:lang="en">DeCAS Ontology</terms:title>
        <vann:preferredNamespacePrefix>decas</vann:preferredNamespacePrefix>
    </owl:Ontology>

    <!-- 
    ///////////////////////////////////////////////////////////////////////////////////////
    //
    // Annotation properties
    //
    ///////////////////////////////////////////////////////////////////////////////////////
     -->

    <!-- http://purl.org/dc/terms/created -->

    <owl:AnnotationProperty rdf:about="http://purl.org/dc/terms/created"/>

    <!-- http://purl.org/dc/terms/description -->

    <owl:AnnotationProperty rdf:about="http://purl.org/dc/terms/description"/>

    <!-- http://purl.org/dc/terms/title -->

    <owl:AnnotationProperty rdf:about="http://purl.org/dc/terms/title"/>

    <!-- http://purl.org/vocab/vann/preferredNamespacePrefix -->

    <owl:AnnotationProperty rdf:about="http://purl.org/vocab/vann/preferredNamespacePrefix"/>

    <!-- http://schema.org/domainIncludes -->

    <owl:AnnotationProperty rdf:about="http://schema.org/domainIncludes"/>

    <!-- http://schema.org/rangeIncludes -->

    <owl:AnnotationProperty rdf:about="http://schema.org/rangeIncludes"/>

    <!-- http://swrl.stanford.edu/ontologies/3.3/swrla.owl#isRuleEnabled -->

    <owl:AnnotationProperty rdf:about="http://swrl.stanford.edu/ontologies/3.3/swrla.owl#isRuleEnabled"/>

    <!-- http://www.w3.org/2004/02/skos/core#definition -->

    <owl:AnnotationProperty rdf:about="http://www.w3.org/2004/02/skos/core#definition"/>

    <!-- http://www.w3.org/2004/02/skos/core#example -->

    <owl:AnnotationProperty rdf:about="http://www.w3.org/2004/02/skos/core#example"/>

    <!-- http://www.w3.org/2004/02/skos/core#note -->

    <owl:AnnotationProperty rdf:about="http://www.w3.org/2004/02/skos/core#note"/>

    <!-- 
    ///////////////////////////////////////////////////////////////////////////////////////
    //
    // Datatypes
    //
    ///////////////////////////////////////////////////////////////////////////////////////
     -->

    <!-- http://www.w3.org/2001/XMLSchema#date -->

    <rdfs:Datatype rdf:about="http://www.w3.org/2001/XMLSchema#date"/>

    <!-- 
    ///////////////////////////////////////////////////////////////////////////////////////
    //
    // Object Properties
    //
    ///////////////////////////////////////////////////////////////////////////////////////
     -->

    <!-- http://www.semanticweb.org/decentralized-context-aware-ontology#has_location -->

    <owl:ObjectProperty rdf:about="http://www.semanticweb.org/decentralized-context-aware-ontology#has_location">
        <owl:equivalentProperty>
            <rdf:Description>
                <owl:inverseOf rdf:resource="http://www.semanticweb.org/decentralized-context-aware-ontology#is_location_of"/>
            </rdf:Description>
        </owl:equivalentProperty>
        <owl:inverseOf rdf:resource="http://www.semanticweb.org/decentralized-context-aware-ontology#is_location_of"/>
        <rdf:type rdf:resource="http://www.w3.org/2002/07/owl#FunctionalProperty"/>
        <rdf:type rdf:resource="http://www.w3.org/2002/07/owl#AsymmetricProperty"/>
        <rdf:type rdf:resource="http://www.w3.org/2002/07/owl#IrreflexiveProperty"/>
        <rdfs:range rdf:resource="http://www.semanticweb.org/decentralized-context-aware-ontology#Location"/>
        <owl:propertyDisjointWith rdf:resource="http://www.semanticweb.org/decentralized-context-aware-ontology#is_located_between"/>
        <rdfs:comment xml:lang="en">Relation between an Actuation or Observation and the Location in which it occurred.</rdfs:comment>
        <rdfs:label xml:lang="en">has location</rdfs:label>
        <skos:definition xml:lang="en">Relation between an Actuation or Observation and the Location in which it occurred.</skos:definition>
    </owl:ObjectProperty>

    <!-- http://www.semanticweb.org/decentralized-context-aware-ontology#is_located_between -->

    <owl:ObjectProperty rdf:about="http://www.semanticweb.org/decentralized-context-aware-ontology#is_located_between">
        <rdf:type rdf:resource="http://www.w3.org/2002/07/owl#AsymmetricProperty"/>
        <rdf:type rdf:resource="http://www.w3.org/2002/07/owl#IrreflexiveProperty"/>
        <rdfs:range rdf:resource="http://www.semanticweb.org/decentralized-context-aware-ontology#Location"/>
        <rdfs:comment xml:lang="en">Relation from an Actuation or Observation to the two Location individuals it connects.</rdfs:comment>
        <rdfs:label xml:lang="en">is located between</rdfs:label>
        <skos:definition xml:lang="en">Relation from an Actuation or Observation to the two Location individuals it connects.</skos:definition>
        <skos:example xml:lang="en">A door connecting two rooms would have two &apos;is located between&apos; properties, defining the two rooms connected by the door.</skos:example>
    </owl:ObjectProperty>

    <!-- http://www.semanticweb.org/decentralized-context-aware-ontology#is_location_of -->

    <owl:ObjectProperty rdf:about="http://www.semanticweb.org/decentralized-context-aware-ontology#is_location_of">
        <rdf:type rdf:resource="http://www.w3.org/2002/07/owl#InverseFunctionalProperty"/>
        <rdf:type rdf:resource="http://www.w3.org/2002/07/owl#AsymmetricProperty"/>
        <rdf:type rdf:resource="http://www.w3.org/2002/07/owl#IrreflexiveProperty"/>
        <rdfs:domain rdf:resource="http://www.semanticweb.org/decentralized-context-aware-ontology#Location"/>
        <rdfs:comment xml:lang="en">Relation between a Location and the Actuation or Observation that occurred there.</rdfs:comment>
        <rdfs:label xml:lang="en">is location of</rdfs:label>
        <skos:definition xml:lang="en">Relation between a Location and the Actuation or Observation that occurred there.</skos:definition>
    </owl:ObjectProperty>

    <!-- http://www.w3.org/ns/sosa/actsOnProperty -->

    <owl:ObjectProperty rdf:about="http://www.w3.org/ns/sosa/actsOnProperty">
        <owl:equivalentProperty>
            <rdf:Description>
                <owl:inverseOf rdf:resource="http://www.w3.org/ns/sosa/isActedOnBy"/>
            </rdf:Description>
        </owl:equivalentProperty>
        <owl:inverseOf rdf:resource="http://www.w3.org/ns/sosa/isActedOnBy"/>
        <rdf:type rdf:resource="http://www.w3.org/2002/07/owl#AsymmetricProperty"/>
        <rdf:type rdf:resource="http://www.w3.org/2002/07/owl#IrreflexiveProperty"/>
        <rdfs:domain rdf:resource="http://www.w3.org/ns/sosa/Actuation"/>
        <rdfs:range rdf:resource="http://www.w3.org/ns/sosa/ActuatableProperty"/>
        <schema:domainIncludes rdf:resource="http://www.w3.org/ns/sosa/Actuation"/>
        <schema:rangeIncludes rdf:resource="http://www.w3.org/ns/sosa/ActuatableProperty"/>
        <rdfs:comment xml:lang="en">Relation between an Actuation and the property of a FeatureOfInterest it is acting upon.</rdfs:comment>
        <rdfs:isDefinedBy rdf:resource="http://www.w3.org/ns/sosa/"/>
        <rdfs:label xml:lang="en">acts on property</rdfs:label>
        <skos:definition xml:lang="en">Relation between an Actuation and the property of a FeatureOfInterest it is acting upon.</skos:definition>
        <skos:example xml:lang="en">In the activity (Actuation) of automatically closing a window if the temperature in a room drops below 20 degrees Celsius, the property on which the Actuator acts upon is the state of the window as it changes from being open to being closed. </skos:example>
    </owl:ObjectProperty>

    <!-- http://www.w3.org/ns/sosa/hasFeatureOfInterest -->

    <owl:ObjectProperty rdf:about="http://www.w3.org/ns/sosa/hasFeatureOfInterest">
        <owl:equivalentProperty>
            <rdf:Description>
                <owl:inverseOf rdf:resource="http://www.w3.org/ns/sosa/isFeatureOfInterestOf"/>
            </rdf:Description>
        </owl:equivalentProperty>
        <owl:inverseOf rdf:resource="http://www.w3.org/ns/sosa/isFeatureOfInterestOf"/>
        <rdf:type rdf:resource="http://www.w3.org/2002/07/owl#AsymmetricProperty"/>
        <rdf:type rdf:resource="http://www.w3.org/2002/07/owl#IrreflexiveProperty"/>
        <rdfs:range rdf:resource="http://www.w3.org/ns/sosa/FeatureOfInterest"/>
        <schema:domainIncludes rdf:resource="http://www.w3.org/ns/sosa/Actuation"/>
        <schema:domainIncludes rdf:resource="http://www.w3.org/ns/sosa/Observation"/>
        <schema:rangeIncludes rdf:resource="http://www.w3.org/ns/sosa/FeatureOfInterest"/>
        <rdfs:comment xml:lang="en">A relation between an Observation and the entity whose quality was observed, or between an Actuation and the entity whose property was modified, or between an act of Sampling and the entity that was sampled.</rdfs:comment>
        <rdfs:isDefinedBy rdf:resource="http://www.w3.org/ns/sosa/"/>
        <rdfs:label xml:lang="en">has feature of interest</rdfs:label>
        <skos:definition xml:lang="en">A relation between an Observation and the entity whose quality was observed, or between an Actuation and the entity whose property was modified, or between an act of Sampling and the entity that was sampled.</skos:definition>
        <skos:example xml:lang="en">For example, in an Observation of the weight of a person, the FeatureOfInterest is the person and the property is its weight.</skos:example>
    </owl:ObjectProperty>

    <!-- http://www.w3.org/ns/sosa/hosts -->

    <owl:ObjectProperty rdf:about="http://www.w3.org/ns/sosa/hosts">
        <owl:equivalentProperty>
            <rdf:Description>
                <owl:inverseOf rdf:resource="http://www.w3.org/ns/sosa/isHostedBy"/>
            </rdf:Description>
        </owl:equivalentProperty>
        <owl:inverseOf rdf:resource="http://www.w3.org/ns/sosa/isHostedBy"/>
        <rdf:type rdf:resource="http://www.w3.org/2002/07/owl#InverseFunctionalProperty"/>
        <rdf:type rdf:resource="http://www.w3.org/2002/07/owl#AsymmetricProperty"/>
        <rdf:type rdf:resource="http://www.w3.org/2002/07/owl#IrreflexiveProperty"/>
        <rdfs:domain rdf:resource="http://www.w3.org/ns/sosa/Platform"/>
        <schema:domainIncludes rdf:resource="http://www.w3.org/ns/sosa/Platform"/>
        <schema:rangeIncludes rdf:resource="http://www.w3.org/ns/sosa/Actuator"/>
        <schema:rangeIncludes rdf:resource="http://www.w3.org/ns/sosa/Platform"/>
        <schema:rangeIncludes rdf:resource="http://www.w3.org/ns/sosa/Sensor"/>
        <rdfs:comment xml:lang="en">Relation between a Platform and a Sensor, Actuator, Sampler, or Platform, hosted or mounted on it.</rdfs:comment>
        <rdfs:isDefinedBy rdf:resource="http://www.w3.org/ns/sosa/"/>
        <rdfs:label xml:lang="en">hosts</rdfs:label>
        <skos:definition xml:lang="en">Relation between a Platform and a Sensor, Actuator, Sampler, or Platform, hosted or mounted on it.</skos:definition>
    </owl:ObjectProperty>

    <!-- http://www.w3.org/ns/sosa/isActedOnBy -->

    <owl:ObjectProperty rdf:about="http://www.w3.org/ns/sosa/isActedOnBy">
        <rdf:type rdf:resource="http://www.w3.org/2002/07/owl#AsymmetricProperty"/>
        <rdf:type rdf:resource="http://www.w3.org/2002/07/owl#IrreflexiveProperty"/>
        <schema:domainIncludes rdf:resource="http://www.w3.org/ns/sosa/ActuatableProperty"/>
        <schema:rangeIncludes rdf:resource="http://www.w3.org/ns/sosa/Actuation"/>
        <rdfs:comment xml:lang="en">Relation between an ActuatableProperty of a FeatureOfInterest and an Actuation changing its state.</rdfs:comment>
        <rdfs:isDefinedBy rdf:resource="http://www.w3.org/ns/sosa/"/>
        <rdfs:label xml:lang="en">is acted on by</rdfs:label>
        <skos:definition xml:lang="en">Relation between an ActuatableProperty of a FeatureOfInterest and an Actuation changing its state.</skos:definition>
        <skos:example xml:lang="en">In the activity (Actuation) of automatically closing a window if the temperature in a room drops below 20 degrees Celsius, the property on which the Actuator acts upon is the state of the window as it changes from being open to being closed. </skos:example>
    </owl:ObjectProperty>

    <!-- http://www.w3.org/ns/sosa/isFeatureOfInterestOf -->

    <owl:ObjectProperty rdf:about="http://www.w3.org/ns/sosa/isFeatureOfInterestOf">
        <rdf:type rdf:resource="http://www.w3.org/2002/07/owl#AsymmetricProperty"/>
        <rdf:type rdf:resource="http://www.w3.org/2002/07/owl#IrreflexiveProperty"/>
        <schema:domainIncludes rdf:resource="http://www.w3.org/ns/sosa/FeatureOfInterest"/>
        <schema:rangeIncludes rdf:resource="http://www.w3.org/ns/sosa/Actuation"/>
        <schema:rangeIncludes rdf:resource="http://www.w3.org/ns/sosa/Observation"/>
        <rdfs:comment xml:lang="en">A relation between a FeatureOfInterest and an Observation about it, an Actuation acting on it, or an act of Sampling that sampled it.</rdfs:comment>
        <rdfs:isDefinedBy rdf:resource="http://www.w3.org/ns/sosa/"/>
        <rdfs:label xml:lang="en">is feature of interest of</rdfs:label>
        <skos:definition xml:lang="en">A relation between a FeatureOfInterest and an Observation about it, an Actuation acting on it, or an act of Sampling that sampled it.</skos:definition>
    </owl:ObjectProperty>

    <!-- http://www.w3.org/ns/sosa/isHostedBy -->

    <owl:ObjectProperty rdf:about="http://www.w3.org/ns/sosa/isHostedBy">
        <rdf:type rdf:resource="http://www.w3.org/2002/07/owl#FunctionalProperty"/>
        <rdf:type rdf:resource="http://www.w3.org/2002/07/owl#AsymmetricProperty"/>
        <rdf:type rdf:resource="http://www.w3.org/2002/07/owl#IrreflexiveProperty"/>
        <schema:domainIncludes rdf:resource="http://www.w3.org/ns/sosa/Actuator"/>
        <schema:domainIncludes rdf:resource="http://www.w3.org/ns/sosa/Platform"/>
        <schema:domainIncludes rdf:resource="http://www.w3.org/ns/sosa/Sensor"/>
        <schema:rangeIncludes rdf:resource="http://www.w3.org/ns/sosa/Platform"/>
        <rdfs:comment xml:lang="en">Relation between a Sensor, Actuator, Sampler, or Platform, and the Platform that it is mounted on or hosted by.</rdfs:comment>
        <rdfs:isDefinedBy rdf:resource="http://www.w3.org/ns/sosa/"/>
        <rdfs:label xml:lang="en">is hosted by</rdfs:label>
        <skos:definition xml:lang="en">Relation between a Sensor, Actuator, Sampler, or Platform, and the Platform that it is mounted on or hosted by.</skos:definition>
    </owl:ObjectProperty>

    <!-- http://www.w3.org/ns/sosa/isObservedBy -->

    <owl:ObjectProperty rdf:about="http://www.w3.org/ns/sosa/isObservedBy">
        <owl:equivalentProperty>
            <rdf:Description>
                <owl:inverseOf rdf:resource="http://www.w3.org/ns/sosa/observes"/>
            </rdf:Description>
        </owl:equivalentProperty>
        <owl:inverseOf rdf:resource="http://www.w3.org/ns/sosa/observes"/>
        <rdf:type rdf:resource="http://www.w3.org/2002/07/owl#AsymmetricProperty"/>
        <rdf:type rdf:resource="http://www.w3.org/2002/07/owl#IrreflexiveProperty"/>
        <rdfs:domain rdf:resource="http://www.w3.org/ns/sosa/ObservableProperty"/>
        <rdfs:range rdf:resource="http://www.w3.org/ns/sosa/Sensor"/>
        <schema:domainIncludes rdf:resource="http://www.w3.org/ns/sosa/ObservableProperty"/>
        <schema:rangeIncludes rdf:resource="http://www.w3.org/ns/sosa/Sensor"/>
        <rdfs:comment xml:lang="en">Relation between an ObservableProperty and the Sensor able to observe it.</rdfs:comment>
        <rdfs:isDefinedBy rdf:resource="http://www.w3.org/ns/sosa/"/>
        <rdfs:label xml:lang="en">is observed by</rdfs:label>
        <skos:definition xml:lang="en">Relation between an ObservableProperty and the Sensor able to observe it.</skos:definition>
    </owl:ObjectProperty>

    <!-- http://www.w3.org/ns/sosa/madeActuation -->

    <owl:ObjectProperty rdf:about="http://www.w3.org/ns/sosa/madeActuation">
        <owl:equivalentProperty>
            <rdf:Description>
                <owl:inverseOf rdf:resource="http://www.w3.org/ns/sosa/madeByActuator"/>
            </rdf:Description>
        </owl:equivalentProperty>
        <owl:inverseOf rdf:resource="http://www.w3.org/ns/sosa/madeByActuator"/>
        <rdf:type rdf:resource="http://www.w3.org/2002/07/owl#InverseFunctionalProperty"/>
        <rdf:type rdf:resource="http://www.w3.org/2002/07/owl#AsymmetricProperty"/>
        <rdf:type rdf:resource="http://www.w3.org/2002/07/owl#IrreflexiveProperty"/>
        <rdfs:domain rdf:resource="http://www.w3.org/ns/sosa/Actuator"/>
        <rdfs:range rdf:resource="http://www.w3.org/ns/sosa/Actuation"/>
        <schema:domainIncludes rdf:resource="http://www.w3.org/ns/sosa/Actuator"/>
        <schema:rangeIncludes rdf:resource="http://www.w3.org/ns/sosa/Actuation"/>
        <rdfs:comment xml:lang="en">Relation between an Actuator and the Actuation it has made.</rdfs:comment>
        <rdfs:isDefinedBy rdf:resource="http://www.w3.org/ns/sosa/"/>
        <rdfs:label xml:lang="en">made actuation</rdfs:label>
        <skos:definition xml:lang="en">Relation between an Actuator and the Actuation it has made.</skos:definition>
    </owl:ObjectProperty>

    <!-- http://www.w3.org/ns/sosa/madeByActuator -->

    <owl:ObjectProperty rdf:about="http://www.w3.org/ns/sosa/madeByActuator">
        <rdf:type rdf:resource="http://www.w3.org/2002/07/owl#FunctionalProperty"/>
        <rdf:type rdf:resource="http://www.w3.org/2002/07/owl#AsymmetricProperty"/>
        <rdf:type rdf:resource="http://www.w3.org/2002/07/owl#IrreflexiveProperty"/>
        <schema:domainIncludes rdf:resource="http://www.w3.org/ns/sosa/Actuation"/>
        <schema:rangeIncludes rdf:resource="http://www.w3.org/ns/sosa/Actuator"/>
        <rdfs:comment xml:lang="en">Relation linking an Actuation to the Actuator that made that Actuation.</rdfs:comment>
        <rdfs:isDefinedBy rdf:resource="http://www.w3.org/ns/sosa/"/>
        <rdfs:label xml:lang="en">made by actuators</rdfs:label>
        <skos:definition xml:lang="en">Relation linking an Actuation to the Actuator that made that Actuation.</skos:definition>
    </owl:ObjectProperty>

    <!-- http://www.w3.org/ns/sosa/madeBySensor -->

    <owl:ObjectProperty rdf:about="http://www.w3.org/ns/sosa/madeBySensor">
        <owl:equivalentProperty>
            <rdf:Description>
                <owl:inverseOf rdf:resource="http://www.w3.org/ns/sosa/madeObservation"/>
            </rdf:Description>
        </owl:equivalentProperty>
        <owl:inverseOf rdf:resource="http://www.w3.org/ns/sosa/madeObservation"/>
        <rdf:type rdf:resource="http://www.w3.org/2002/07/owl#FunctionalProperty"/>
        <rdf:type rdf:resource="http://www.w3.org/2002/07/owl#AsymmetricProperty"/>
        <rdf:type rdf:resource="http://www.w3.org/2002/07/owl#IrreflexiveProperty"/>
        <rdfs:domain rdf:resource="http://www.w3.org/ns/sosa/Observation"/>
        <rdfs:range rdf:resource="http://www.w3.org/ns/sosa/Sensor"/>
        <schema:domainIncludes rdf:resource="http://www.w3.org/ns/sosa/Observation"/>
        <schema:rangeIncludes rdf:resource="http://www.w3.org/ns/sosa/Sensor"/>
        <rdfs:comment xml:lang="en">Relation between an Observation and the Sensor which made the Observation.</rdfs:comment>
        <rdfs:isDefinedBy rdf:resource="http://www.w3.org/ns/sosa/"/>
        <rdfs:label xml:lang="en">made by sensor</rdfs:label>
        <skos:definition xml:lang="en">Relation between an Observation and the Sensor which made the Observation.</skos:definition>
    </owl:ObjectProperty>

    <!-- http://www.w3.org/ns/sosa/madeObservation -->

    <owl:ObjectProperty rdf:about="http://www.w3.org/ns/sosa/madeObservation">
        <rdf:type rdf:resource="http://www.w3.org/2002/07/owl#InverseFunctionalProperty"/>
        <rdf:type rdf:resource="http://www.w3.org/2002/07/owl#AsymmetricProperty"/>
        <rdf:type rdf:resource="http://www.w3.org/2002/07/owl#IrreflexiveProperty"/>
        <schema:domainIncludes rdf:resource="http://www.w3.org/ns/sosa/Sensor"/>
        <schema:rangeIncludes rdf:resource="http://www.w3.org/ns/sosa/Observation"/>
        <rdfs:comment xml:lang="en">Relation between a Sensor and an Observation made by the Sensor.</rdfs:comment>
        <rdfs:isDefinedBy rdf:resource="http://www.w3.org/ns/sosa/"/>
        <rdfs:label xml:lang="en">made observation</rdfs:label>
        <skos:definition xml:lang="en">Relation between a Sensor and an Observation made by the Sensor.</skos:definition>
    </owl:ObjectProperty>

    <!-- http://www.w3.org/ns/sosa/observedProperty -->

    <owl:ObjectProperty rdf:about="http://www.w3.org/ns/sosa/observedProperty">
        <rdf:type rdf:resource="http://www.w3.org/2002/07/owl#FunctionalProperty"/>
        <rdf:type rdf:resource="http://www.w3.org/2002/07/owl#AsymmetricProperty"/>
        <rdf:type rdf:resource="http://www.w3.org/2002/07/owl#IrreflexiveProperty"/>
        <rdfs:domain rdf:resource="http://www.w3.org/ns/sosa/Observation"/>
        <rdfs:range rdf:resource="http://www.w3.org/ns/sosa/ObservableProperty"/>
        <schema:domainIncludes rdf:resource="http://www.w3.org/ns/sosa/Observation"/>
        <schema:rangeIncludes rdf:resource="http://www.w3.org/ns/sosa/ObservableProperty"/>
        <rdfs:comment xml:lang="en">Relation linking an Observation to the property that was observed. The ObservableProperty should be a property of the FeatureOfInterest (linked by hasFeatureOfInterest) of this Observation.</rdfs:comment>
        <rdfs:isDefinedBy rdf:resource="http://www.w3.org/ns/sosa/"/>
        <rdfs:label xml:lang="en">observed property</rdfs:label>
        <skos:definition xml:lang="en">Relation linking an Observation to the property that was observed. The ObservableProperty should be a property of the FeatureOfInterest (linked by hasFeatureOfInterest) of this Observation.</skos:definition>
    </owl:ObjectProperty>

    <!-- http://www.w3.org/ns/sosa/observes -->

    <owl:ObjectProperty rdf:about="http://www.w3.org/ns/sosa/observes">
        <rdfs:subPropertyOf rdf:resource="http://www.w3.org/ns/ssn/forProperty"/>
        <rdf:type rdf:resource="http://www.w3.org/2002/07/owl#AsymmetricProperty"/>
        <rdf:type rdf:resource="http://www.w3.org/2002/07/owl#IrreflexiveProperty"/>
        <schema:domainIncludes rdf:resource="http://www.w3.org/ns/sosa/Sensor"/>
        <schema:rangeIncludes rdf:resource="http://www.w3.org/ns/sosa/ObservableProperty"/>
        <rdfs:comment xml:lang="en">Relation between a Sensor and an ObservableProperty that it is capable of sensing.</rdfs:comment>
        <rdfs:isDefinedBy rdf:resource="http://www.w3.org/ns/sosa/"/>
        <rdfs:label xml:lang="en">observes</rdfs:label>
        <skos:definition xml:lang="en">Relation between a Sensor and an ObservableProperty that it is capable of sensing.</skos:definition>
    </owl:ObjectProperty>


    <!-- http://www.w3.org/ns/ssn/forProperty -->

    <owl:ObjectProperty rdf:about="http://www.w3.org/ns/ssn/forProperty">
        <rdfs:comment xml:lang="en">A relation between some aspect of an entity and a Property.</rdfs:comment>
        <rdfs:isDefinedBy rdf:resource="http://www.w3.org/ns/ssn/"/>
        <rdfs:label xml:lang="en">for property</rdfs:label>
        <skos:definition xml:lang="en">A relation between some aspect of an entity and a Property.</skos:definition>
        <skos:example xml:lang="en">For example, from a Sensor to the properties it can observe; from an Actuator to the properties it can act on; from a Deployment to the properties it was installed to observe or act on; from a SystemCapability to the Property the capability is described for.</skos:example>
    </owl:ObjectProperty>

    <!-- http://www.w3.org/ns/ssn/hasProperty -->

    <owl:ObjectProperty rdf:about="http://www.w3.org/ns/ssn/hasProperty">
        <owl:equivalentProperty>
            <rdf:Description>
                <owl:inverseOf rdf:resource="http://www.w3.org/ns/ssn/isPropertyOf"/>
            </rdf:Description>
        </owl:equivalentProperty>
        <owl:inverseOf rdf:resource="http://www.w3.org/ns/ssn/isPropertyOf"/>
        <rdf:type rdf:resource="http://www.w3.org/2002/07/owl#AsymmetricProperty"/>
        <rdf:type rdf:resource="http://www.w3.org/2002/07/owl#IrreflexiveProperty"/>
        <rdfs:comment xml:lang="en">Relation between an entity and a Property of that entity.</rdfs:comment>
        <rdfs:isDefinedBy rdf:resource="http://www.w3.org/ns/ssn/"/>
        <rdfs:label xml:lang="en">has property</rdfs:label>
        <skos:definition xml:lang="en">Relation between an entity and a Property of that entity.</skos:definition>
    </owl:ObjectProperty>

    <!-- http://www.w3.org/ns/ssn/isPropertyOf -->

    <owl:ObjectProperty rdf:about="http://www.w3.org/ns/ssn/isPropertyOf">
        <rdf:type rdf:resource="http://www.w3.org/2002/07/owl#AsymmetricProperty"/>
        <rdf:type rdf:resource="http://www.w3.org/2002/07/owl#IrreflexiveProperty"/>
        <rdfs:domain rdf:resource="http://www.w3.org/ns/ssn/Property"/>
        <rdfs:comment xml:lang="en">Relation between a Property and the entity it belongs to.</rdfs:comment>
        <rdfs:isDefinedBy rdf:resource="http://www.w3.org/ns/ssn/"/>
        <rdfs:label xml:lang="en">is property of</rdfs:label>
        <skos:definition xml:lang="en">Relation between a Property and the entity it belongs to.</skos:definition>
    </owl:ObjectProperty>

    <!-- 
    ///////////////////////////////////////////////////////////////////////////////////////
    //
    // Data properties
    //
    ///////////////////////////////////////////////////////////////////////////////////////
     -->

    <!-- http://www.semanticweb.org/decentralized-context-aware-ontology#has_limit -->

    <owl:DatatypeProperty rdf:about="http://www.semanticweb.org/decentralized-context-aware-ontology#has_limit">
        <rdf:type rdf:resource="http://www.w3.org/2002/07/owl#FunctionalProperty"/>
        <rdfs:domain rdf:resource="http://www.w3.org/ns/sosa/Sensor"/>
        <rdfs:range rdf:resource="http://www.w3.org/2001/XMLSchema#integer"/>
        <rdfs:comment xml:lang="en">Allowed limit of a Sensor reading before an alert should be triggered.</rdfs:comment>
        <rdfs:label xml:lang="en">has limit</rdfs:label>
        <skos:definition xml:lang="en">Allowed limit of a Sensor reading before an alert should be triggered.</skos:definition>
    </owl:DatatypeProperty>

    <!-- http://www.semanticweb.org/decentralized-context-aware-ontology#min_temperature -->

    <owl:DatatypeProperty rdf:about="http://www.semanticweb.org/decentralized-context-aware-ontology#min_temperature">
        <rdf:type rdf:resource="http://www.w3.org/2002/07/owl#FunctionalProperty"/>
        <rdfs:domain rdf:resource="http://www.semanticweb.org/decentralized-context-aware-ontology#Material"/>
        <rdfs:range rdf:datatype="http://www.w3.org/2001/XMLSchema#decimal"/>
        <rdfs:comment xml:lang="en">Minimum allowed temperature for materials.</rdfs:comment>
        <rdfs:label xml:lang="en">Minimum Temperature</rdfs:label>
        <skos:definition xml:lang="en">Minimum allowed temperature for materials.</skos:definition>
    </owl:DatatypeProperty>

    <!-- http://www.semanticweb.org/decentralized-context-aware-ontology#max_temperature -->

    <owl:DatatypeProperty rdf:about="http://www.semanticweb.org/decentralized-context-aware-ontology#min_temperature">
        <rdf:type rdf:resource="http://www.w3.org/2002/07/owl#FunctionalProperty"/>
        <rdfs:domain rdf:resource="http://www.semanticweb.org/decentralized-context-aware-ontology#Material"/>
        <rdfs:range rdf:datatype="http://www.w3.org/2001/XMLSchema#decimal"/>
        <rdfs:comment xml:lang="en">Maximum allowed temperature for materials.</rdfs:comment>
        <rdfs:label xml:lang="en">Maximum Temperature</rdfs:label>
        <skos:definition xml:lang="en">Maximum allowed temperature for materials.</skos:definition>
    </owl:DatatypeProperty>

    <!-- http://www.semanticweb.org/decentralized-context-aware-ontology#has_on_state -->

    <owl:DatatypeProperty rdf:about="http://www.semanticweb.org/decentralized-context-aware-ontology#has_on_state">
        <rdf:type rdf:resource="http://www.w3.org/2002/07/owl#FunctionalProperty"/>
        <rdfs:domain rdf:resource="http://www.w3.org/ns/sosa/Actuation"/>
        <rdfs:range rdf:resource="http://www.w3.org/2001/XMLSchema#boolean"/>
        <rdfs:comment xml:lang="en">The state of an actuation event which operates on a feature of interest Switch property.</rdfs:comment>
        <rdfs:label xml:lang="en">has on state</rdfs:label>
        <skos:definition xml:lang="en">The state of an actuation event which operates on a feature of interest Switch property.</skos:definition>
    </owl:DatatypeProperty>

    <!-- http://www.semanticweb.org/decentralized-context-aware-ontology#is_active -->

    <owl:DatatypeProperty rdf:about="http://www.semanticweb.org/decentralized-context-aware-ontology#is_active">
        <rdf:type rdf:resource="http://www.w3.org/2002/07/owl#FunctionalProperty"/>
        <rdfs:domain rdf:resource="http://www.w3.org/ns/ssn/System"/>
        <rdfs:range rdf:resource="http://www.w3.org/2001/XMLSchema#boolean"/>
        <rdfs:comment xml:lang="en">The active state of a Platform. Intended to be linked to systems which have a switchable state.</rdfs:comment>
        <rdfs:label xml:lang="en">is active</rdfs:label>
        <skos:definition xml:lang="en">The active state of a Platform. Intended to be linked to systems which have a switchable state.</skos:definition>
    </owl:DatatypeProperty>

    <!-- http://www.semanticweb.org/decentralized-context-aware-ontology#is_established -->

    <owl:DatatypeProperty rdf:about="http://www.semanticweb.org/decentralized-context-aware-ontology#is_established">
        <rdf:type rdf:resource="http://www.w3.org/2002/07/owl#FunctionalProperty"/>
        <rdfs:domain rdf:resource="http://www.w3.org/ns/sosa/Platform"/>
        <rdfs:range rdf:resource="http://www.w3.org/2001/XMLSchema#boolean"/>
        <rdfs:comment xml:lang="en">The state of connectivity of a device to the systems.</rdfs:comment>
        <rdfs:label xml:lang="en">is established</rdfs:label>
        <skos:definition xml:lang="en">The state of connectivity of a device to the systems.</skos:definition>
    </owl:DatatypeProperty>

    <!-- http://www.semanticweb.org/decentralized-context-aware-ontology#is_on -->

    <owl:DatatypeProperty rdf:about="http://www.semanticweb.org/decentralized-context-aware-ontology#is_on">
        <rdf:type rdf:resource="http://www.w3.org/2002/07/owl#FunctionalProperty"/>
        <rdfs:domain rdf:resource="http://www.semanticweb.org/decentralized-context-aware-ontology#Switch_Actuator"/>
        <rdfs:range rdf:resource="http://www.w3.org/2001/XMLSchema#boolean"/>
        <rdfs:comment xml:lang="en">The state of a feature of interest Switch property or Platform.</rdfs:comment>
        <rdfs:label xml:lang="en">is on</rdfs:label>
        <skos:definition xml:lang="en">The state of a feature of interest Switch property or Platform.</skos:definition>
    </owl:DatatypeProperty>
    


    <!-- http://www.w3.org/ns/sosa/hasSimpleResult -->

    <owl:DatatypeProperty rdf:about="http://www.w3.org/ns/sosa/hasSimpleResult">
        <rdf:type rdf:resource="http://www.w3.org/2002/07/owl#FunctionalProperty"/>
        <schema:domainIncludes rdf:resource="http://www.w3.org/ns/sosa/Actuation"/>
        <schema:domainIncludes rdf:resource="http://www.w3.org/ns/sosa/Observation"/>
        <rdfs:comment xml:lang="en">The simple value of an Observation or Actuation or act of Sampling.</rdfs:comment>
        <rdfs:isDefinedBy rdf:resource="http://www.w3.org/ns/sosa/"/>
        <rdfs:label xml:lang="en">has simple result</rdfs:label>
        <skos:definition xml:lang="en">The simple value of an Observation or Actuation or act of Sampling.</skos:definition>
        <skos:example xml:lang="en">For instance, the values 23 or true.</skos:example>
    </owl:DatatypeProperty>
    


    <!-- http://www.w3.org/ns/sosa/resultTime -->

    <owl:DatatypeProperty rdf:about="http://www.w3.org/ns/sosa/resultTime">
        <rdf:type rdf:resource="http://www.w3.org/2002/07/owl#FunctionalProperty"/>
        <rdfs:range rdf:resource="http://www.w3.org/2001/XMLSchema#dateTime"/>
        <schema:domainIncludes rdf:resource="http://www.w3.org/ns/sosa/Actuation"/>
        <schema:domainIncludes rdf:resource="http://www.w3.org/ns/sosa/Observation"/>
        <rdfs:comment xml:lang="en">The result time is the instant of time when the Observation, Actuation or Sampling activity was completed.</rdfs:comment>
        <rdfs:isDefinedBy rdf:resource="http://www.w3.org/ns/sosa/"/>
        <rdfs:label xml:lang="en">result time</rdfs:label>
        <skos:definition xml:lang="en">The result time is the instant of time when the Observation, Actuation or Sampling activity was completed.</skos:definition>
    </owl:DatatypeProperty>
    


    <!-- 
    ///////////////////////////////////////////////////////////////////////////////////////
    //
    // Classes
    //
    ///////////////////////////////////////////////////////////////////////////////////////
     -->

    <!-- http://www.semanticweb.org/decentralized-context-aware-ontology#Agitator -->

    <owl:Class rdf:about="http://www.semanticweb.org/decentralized-context-aware-ontology#Agitator">
        <rdfs:subClassOf rdf:resource="http://www.w3.org/ns/sosa/FeatureOfInterest"/>
        <rdfs:subClassOf>
            <owl:Restriction>
                <owl:onProperty rdf:resource="http://www.w3.org/ns/ssn/hasProperty"/>
                <owl:allValuesFrom rdf:resource="http://www.semanticweb.org/decentralized-context-aware-ontology#Switch"/>
            </owl:Restriction>
        </rdfs:subClassOf>
        <rdfs:comment xml:lang="en">A device that is responsible for blending materials.</rdfs:comment>
        <rdfs:label xml:lang="en">Agitator</rdfs:label>
        <skos:definition xml:lang="en">A device that is responsible for blending materials.</skos:definition>
    </owl:Class>

    <!-- http://www.semanticweb.org/decentralized-context-aware-ontology#Flash_Mixer_Machine -->

    <owl:Class rdf:about="http://www.semanticweb.org/decentralized-context-aware-ontology#Flash_Mixer_Machine">
        <owl:equivalentClass>
            <owl:Class>
                <owl:intersectionOf rdf:parseType="Collection">
                    <rdf:Description rdf:about="http://www.w3.org/ns/sosa/Platform"/>
                    <owl:Restriction>
                        <owl:onProperty rdf:resource="http://www.w3.org/ns/sosa/hosts"/>
                        <owl:someValuesFrom rdf:resource="http://www.semanticweb.org/decentralized-context-aware-ontology#Switch_Actuator"/>
                    </owl:Restriction>
                    <owl:Restriction>
                        <owl:onProperty rdf:resource="http://www.w3.org/ns/sosa/hosts"/>
                        <owl:someValuesFrom rdf:resource="http://www.semanticweb.org/decentralized-context-aware-ontology#Material_Sensor"/>
                    </owl:Restriction>
                </owl:intersectionOf>
            </owl:Class>
        </owl:equivalentClass>
        <rdfs:label xml:lang="en">Flash Mixer Machine</rdfs:label>
    </owl:Class>

    <!-- http://www.semanticweb.org/decentralized-context-aware-ontology#Location -->

    <owl:Class rdf:about="http://www.semanticweb.org/decentralized-context-aware-ontology#Location">
        <rdfs:subClassOf>
            <owl:Restriction>
                <owl:onProperty rdf:resource="http://www.semanticweb.org/decentralized-context-aware-ontology#is_location_of"/>
                <owl:someValuesFrom rdf:resource="http://www.w3.org/ns/sosa/Platform"/>
            </owl:Restriction>
        </rdfs:subClassOf>
        <rdfs:subClassOf>
            <owl:Restriction>
                <owl:onProperty rdf:resource="http://www.semanticweb.org/decentralized-context-aware-ontology#is_location_of"/>
                <owl:someValuesFrom rdf:resource="http://www.w3.org/ns/ssn/System"/>
            </owl:Restriction>
        </rdfs:subClassOf>
        <rdfs:comment xml:lang="en">Location where either a Sensor, Actuator or Platform (which hosts Sensors and Actuators) can be found.</rdfs:comment>
        <rdfs:label xml:lang="en">Location</rdfs:label>
        <skos:definition xml:lang="en">Location where either a Sensor, Actuator or Platform (which hosts Sensors and Actuators) can be found.</skos:definition>
    </owl:Class>

    <!-- http://www.semanticweb.org/decentralized-context-aware-ontology#Material -->

    <owl:Class rdf:about="http://www.semanticweb.org/decentralized-context-aware-ontology#Material">
        <rdfs:subClassOf rdf:resource="http://www.w3.org/ns/sosa/FeatureOfInterest"/>
        <rdfs:subClassOf>
            <owl:Restriction>
                <owl:onProperty rdf:resource="http://www.w3.org/ns/ssn/hasProperty"/>
                <owl:allValuesFrom rdf:resource="http://www.semanticweb.org/decentralized-context-aware-ontology#Temperature"/>
            </owl:Restriction>
        </rdfs:subClassOf>
        <rdfs:comment xml:lang="en">A substance made up of various types of particles that occupy physical space and have inertia.</rdfs:comment>
        <rdfs:label xml:lang="en">Material</rdfs:label>
        <skos:definition xml:lang="en">A substance made up of various types of particles that occupy physical space and have inertia.</skos:definition>
    </owl:Class>

    <!-- http://www.semanticweb.org/decentralized-context-aware-ontology#Material_Observation -->

    <owl:Class rdf:about="http://www.semanticweb.org/decentralized-context-aware-ontology#Material_Observation">
        <owl:equivalentClass>
            <owl:Class>
                <owl:intersectionOf rdf:parseType="Collection">
                    <rdf:Description rdf:about="http://www.w3.org/ns/sosa/Observation"/>
                    <owl:Restriction>
                        <owl:onProperty rdf:resource="http://www.w3.org/ns/sosa/hasFeatureOfInterest"/>
                        <owl:allValuesFrom>
                            <owl:Class>
                                <owl:unionOf rdf:parseType="Collection">
                                    <rdf:Description rdf:about="http://www.semanticweb.org/decentralized-context-aware-ontology#Material"/>
                                </owl:unionOf>
                            </owl:Class>
                        </owl:allValuesFrom>
                    </owl:Restriction>
                </owl:intersectionOf>
            </owl:Class>
        </owl:equivalentClass>
        <owl:equivalentClass>
            <owl:Restriction>
                <owl:onProperty rdf:resource="http://www.w3.org/ns/sosa/observedProperty"/>
                <owl:qualifiedCardinality rdf:datatype="http://www.w3.org/2001/XMLSchema#nonNegativeInteger">1</owl:qualifiedCardinality>
                <owl:onClass rdf:resource="http://www.semanticweb.org/decentralized-context-aware-ontology#Material_Property"/>
            </owl:Restriction>
        </owl:equivalentClass>
        <rdfs:comment xml:lang="en">Observations relating to a material properties in an area.</rdfs:comment>
        <rdfs:label xml:lang="en">Material Observation</rdfs:label>
        <skos:definition xml:lang="en">Observations relating to a material properties in an area.</skos:definition>
    </owl:Class>

    <!-- http://www.semanticweb.org/decentralized-context-aware-ontology#Material_Property -->

    <owl:Class rdf:about="http://www.semanticweb.org/decentralized-context-aware-ontology#Material_Property">
        <rdfs:subClassOf rdf:resource="http://www.w3.org/ns/sosa/ObservableProperty"/>
        <rdfs:comment xml:lang="en">An observable property found in a material.</rdfs:comment>
        <rdfs:label xml:lang="en">Material Property</rdfs:label>
        <skos:definition xml:lang="en">An observable property found in a material.</skos:definition>
    </owl:Class>

    <!-- http://www.semanticweb.org/decentralized-context-aware-ontology#Material_Sensor -->

    <owl:Class rdf:about="http://www.semanticweb.org/decentralized-context-aware-ontology#Material_Sensor">
        <rdfs:subClassOf rdf:resource="http://www.w3.org/ns/sosa/Sensor"/>
        <rdfs:subClassOf>
            <owl:Restriction>
                <owl:onProperty rdf:resource="http://www.w3.org/ns/sosa/madeObservation"/>
                <owl:allValuesFrom rdf:resource="http://www.semanticweb.org/decentralized-context-aware-ontology#Material_Observation"/>
            </owl:Restriction>
        </rdfs:subClassOf>
        <rdfs:subClassOf>
            <owl:Restriction>
                <owl:onProperty rdf:resource="http://www.w3.org/ns/sosa/observedProperty"/>
                <owl:allValuesFrom rdf:resource="http://www.semanticweb.org/decentralized-context-aware-ontology#Material_Property"/>
            </owl:Restriction>
        </rdfs:subClassOf>
        <rdfs:comment xml:lang="en">A type of sensor is used to measure materials conditions. Examples could include humidity, temperature or pollution sensors.</rdfs:comment>
        <rdfs:label xml:lang="en">Material Sensor</rdfs:label>
        <skos:definition xml:lang="en">A type of sensor used to measure environmental conditions. Examples could include humidity, temperature or pollution sensors.</skos:definition>
        <skos:example xml:lang="en">A sensor used to measure the temperature of the atmosphere in a room.</skos:example>
    </owl:Class>

    <!-- http://www.semanticweb.org/decentralized-context-aware-ontology#Mixer_Agitator_Actuation -->

    <owl:Class rdf:about="http://www.semanticweb.org/decentralized-context-aware-ontology#Mixer_Agitator_Actuation">
        <rdfs:subClassOf rdf:resource="http://www.w3.org/ns/sosa/Actuation"/>
        <rdfs:subClassOf>
            <owl:Restriction>
                <owl:onProperty rdf:resource="http://www.w3.org/ns/sosa/hasFeatureOfInterest"/>
                <owl:allValuesFrom rdf:resource="http://www.semanticweb.org/decentralized-context-aware-ontology#Processing_Material"/>
            </owl:Restriction>
        </rdfs:subClassOf>
        <rdfs:comment xml:lang="en">Actuation events which occur on a mixer&apos;s agitator.</rdfs:comment>
        <rdfs:label xml:lang="en">Agitator Actuation</rdfs:label>
        <skos:definition xml:lang="en">Actuation events which occur on a mixer&apos;s agitator.</skos:definition>
    </owl:Class>

    <!-- http://www.semanticweb.org/decentralized-context-aware-ontology#Processing_Material -->

    <owl:Class rdf:about="http://www.semanticweb.org/decentralized-context-aware-ontology#Processing_Material">
        <rdfs:subClassOf rdf:resource="http://www.semanticweb.org/decentralized-context-aware-ontology#Material"/>
        <owl:disjointWith rdf:resource="http://www.semanticweb.org/decentralized-context-aware-ontology#Product"/>
        <owl:disjointWith rdf:resource="http://www.semanticweb.org/decentralized-context-aware-ontology#Raw_Material"/>
        <rdfs:comment xml:lang="en">A material is produced during the production process.</rdfs:comment>
        <rdfs:label xml:lang="en">Processing Material</rdfs:label>
        <skos:definition xml:lang="en">A material is used to produce the final product.</skos:definition>
    </owl:Class>

    <!-- http://www.semanticweb.org/decentralized-context-aware-ontology#Product -->

    <owl:Class rdf:about="http://www.semanticweb.org/decentralized-context-aware-ontology#Product">
        <rdfs:subClassOf rdf:resource="http://www.semanticweb.org/decentralized-context-aware-ontology#Material"/>
        <owl:disjointWith rdf:resource="http://www.semanticweb.org/decentralized-context-aware-ontology#Raw_Material"/>
        <rdfs:comment xml:lang="en">A material is used to produce the final product.</rdfs:comment>
        <rdfs:label xml:lang="en">Product</rdfs:label>
        <skos:definition xml:lang="en">A material is used to produce the final product.</skos:definition>
    </owl:Class>

    <!-- http://www.semanticweb.org/decentralized-context-aware-ontology#Raw_Material -->

    <owl:Class rdf:about="http://www.semanticweb.org/decentralized-context-aware-ontology#Raw_Material">
        <rdfs:subClassOf rdf:resource="http://www.semanticweb.org/decentralized-context-aware-ontology#Material"/>
        <rdfs:comment xml:lang="en">A material is used to produce the final product.</rdfs:comment>
        <rdfs:label xml:lang="en">Raw Material</rdfs:label>
        <skos:definition xml:lang="en">A material is used to produce the final product.</skos:definition>
    </owl:Class>

    <!-- http://www.semanticweb.org/decentralized-context-aware-ontology#Switch -->

    <owl:Class rdf:about="http://www.semanticweb.org/decentralized-context-aware-ontology#Switch">
        <rdfs:subClassOf rdf:resource="http://www.w3.org/ns/sosa/ActuatableProperty"/>
        <rdfs:subClassOf>
            <owl:Restriction>
                <owl:onProperty rdf:resource="http://www.w3.org/ns/ssn/isPropertyOf"/>
                <owl:someValuesFrom rdf:resource="http://www.semanticweb.org/decentralized-context-aware-ontology#Agitator"/>
            </owl:Restriction>
        </rdfs:subClassOf>
        <rdfs:subClassOf>
            <owl:Restriction>
                <owl:onProperty rdf:resource="http://www.w3.org/ns/sosa/isActedOnBy"/>
                <owl:allValuesFrom rdf:resource="http://www.semanticweb.org/decentralized-context-aware-ontology#Switch_Actuator"/>
            </owl:Restriction>
        </rdfs:subClassOf>
        <rdfs:comment xml:lang="en">An actuation property relating to the state or level of a switchable actuators.</rdfs:comment>
        <rdfs:label xml:lang="en">Switch</rdfs:label>
        <skos:definition xml:lang="en">An actuation property relating to the state or level of a switchable actuators.</skos:definition>
    </owl:Class>

    <!-- http://www.semanticweb.org/decentralized-context-aware-ontology#Switch_Actuator -->

    <owl:Class rdf:about="http://www.semanticweb.org/decentralized-context-aware-ontology#Switch_Actuator">
        <owl:equivalentClass>
            <owl:Class>
                <owl:intersectionOf rdf:parseType="Collection">
                    <rdf:Description rdf:about="http://www.w3.org/ns/sosa/Actuator"/>
                    <owl:Restriction>
                        <owl:onProperty rdf:resource="http://www.w3.org/ns/ssn/forProperty"/>
                        <owl:allValuesFrom rdf:resource="http://www.semanticweb.org/decentralized-context-aware-ontology#Switch"/>
                    </owl:Restriction>
                </owl:intersectionOf>
            </owl:Class>
        </owl:equivalentClass>
        <rdfs:comment xml:lang="en">An actuators is used to change the state of a switchable property.</rdfs:comment>
        <rdfs:label xml:lang="en">Switch Actuator</rdfs:label>
        <skos:definition xml:lang="en">An actuators is used to change the state of a switchable property.</skos:definition>
    </owl:Class>

    <!-- http://www.semanticweb.org/decentralized-context-aware-ontology#Temperature -->

    <owl:Class rdf:about="http://www.semanticweb.org/decentralized-context-aware-ontology#Temperature">
        <rdfs:subClassOf rdf:resource="http://www.semanticweb.org/decentralized-context-aware-ontology#Material_Property"/>
        <rdfs:subClassOf>
            <owl:Restriction>
                <owl:onProperty rdf:resource="http://www.w3.org/ns/sosa/isObservedBy"/>
                <owl:allValuesFrom rdf:resource="http://www.semanticweb.org/decentralized-context-aware-ontology#Temperature_Sensor"/>
            </owl:Restriction>
        </rdfs:subClassOf>
        <rdfs:comment xml:lang="en">Temperature is a measure of the infrared energy held by a feature of interest.</rdfs:comment>
        <rdfs:label xml:lang="en">Temperature</rdfs:label>
        <skos:definition xml:lang="en">Temperature is a measure of the infrared energy held by a feature of interest.</skos:definition>
    </owl:Class>

    <!-- http://www.semanticweb.org/decentralized-context-aware-ontology#Temperature_Sensor -->

    <owl:Class rdf:about="http://www.semanticweb.org/decentralized-context-aware-ontology#Temperature_Sensor">
        <owl:equivalentClass>
            <owl:Class>
                <owl:intersectionOf rdf:parseType="Collection">
                    <rdf:Description rdf:about="http://www.semanticweb.org/decentralized-context-aware-ontology#Material_Sensor"/>
                    <owl:Restriction>
                        <owl:onProperty rdf:resource="http://www.w3.org/ns/sosa/observes"/>
                        <owl:allValuesFrom rdf:resource="http://www.semanticweb.org/decentralized-context-aware-ontology#Temperature"/>
                    </owl:Restriction>
                </owl:intersectionOf>
            </owl:Class>
        </owl:equivalentClass>
        <rdfs:comment xml:lang="en">A sensor that detects the temperature of a material.</rdfs:comment>
        <rdfs:label xml:lang="en">Temperature Sensor</rdfs:label>
        <skos:definition xml:lang="en">A sensor that detects the temperature of a material.</skos:definition>
    </owl:Class>

    <!-- http://www.w3.org/ns/sosa/ActuatableProperty -->

    <owl:Class rdf:about="http://www.w3.org/ns/sosa/ActuatableProperty">
        <rdfs:subClassOf rdf:resource="http://www.w3.org/ns/ssn/Property"/>
        <rdfs:subClassOf>
            <owl:Restriction>
                <owl:onProperty rdf:resource="http://www.w3.org/ns/sosa/isActedOnBy"/>
                <owl:allValuesFrom rdf:resource="http://www.w3.org/ns/sosa/Actuation"/>
            </owl:Restriction>
        </rdfs:subClassOf>
        <rdfs:comment xml:lang="en">An actuatable quality (property, characteristic) of a FeatureOfInterest.</rdfs:comment>
        <rdfs:isDefinedBy rdf:resource="http://www.w3.org/ns/sosa/"/>
        <rdfs:label xml:lang="en">Actuatable Property</rdfs:label>
        <skos:definition xml:lang="en">An actuatable quality (property, characteristic) of a FeatureOfInterest.</skos:definition>
        <skos:example xml:lang="en">A window actuators acts by changing the state between a frame and a window. The ability of the window to be opened and closed is its ActuatableProperty.</skos:example>
    </owl:Class>

    <!-- http://www.w3.org/ns/sosa/Actuation -->

    <owl:Class rdf:about="http://www.w3.org/ns/sosa/Actuation">
        <rdfs:subClassOf>
            <owl:Restriction>
                <owl:onProperty rdf:resource="http://www.w3.org/ns/sosa/actsOnProperty"/>
                <owl:allValuesFrom rdf:resource="http://www.w3.org/ns/sosa/ActuatableProperty"/>
            </owl:Restriction>
        </rdfs:subClassOf>
        <rdfs:subClassOf>
            <owl:Restriction>
                <owl:onProperty rdf:resource="http://www.w3.org/ns/sosa/hasFeatureOfInterest"/>
                <owl:allValuesFrom rdf:resource="http://www.w3.org/ns/sosa/FeatureOfInterest"/>
            </owl:Restriction>
        </rdfs:subClassOf>
        <rdfs:subClassOf>
            <owl:Restriction>
                <owl:onProperty rdf:resource="http://www.w3.org/ns/sosa/madeByActuator"/>
                <owl:allValuesFrom rdf:resource="http://www.w3.org/ns/sosa/Actuator"/>
            </owl:Restriction>
        </rdfs:subClassOf>
        <rdfs:subClassOf>
            <owl:Restriction>
                <owl:onProperty rdf:resource="http://www.w3.org/ns/sosa/actsOnProperty"/>
                <owl:minCardinality rdf:datatype="http://www.w3.org/2001/XMLSchema#nonNegativeInteger">1</owl:minCardinality>
            </owl:Restriction>
        </rdfs:subClassOf>
        <rdfs:subClassOf>
            <owl:Restriction>
                <owl:onProperty rdf:resource="http://www.w3.org/ns/sosa/hasFeatureOfInterest"/>
                <owl:cardinality rdf:datatype="http://www.w3.org/2001/XMLSchema#nonNegativeInteger">1</owl:cardinality>
            </owl:Restriction>
        </rdfs:subClassOf>
        <rdfs:subClassOf>
            <owl:Restriction>
                <owl:onProperty rdf:resource="http://www.w3.org/ns/sosa/madeByActuator"/>
                <owl:cardinality rdf:datatype="http://www.w3.org/2001/XMLSchema#nonNegativeInteger">1</owl:cardinality>
            </owl:Restriction>
        </rdfs:subClassOf>
        <rdfs:subClassOf>
            <owl:Restriction>
                <owl:onProperty rdf:resource="http://www.w3.org/ns/sosa/resultTime"/>
                <owl:cardinality rdf:datatype="http://www.w3.org/2001/XMLSchema#nonNegativeInteger">1</owl:cardinality>
            </owl:Restriction>
        </rdfs:subClassOf>
        <rdfs:comment xml:lang="en">An Actuation carries out an (Actuation) Procedure to change the state of the world using an Actuator.</rdfs:comment>
        <rdfs:isDefinedBy rdf:resource="http://www.w3.org/ns/sosa/"/>
        <rdfs:label xml:lang="en">Actuation</rdfs:label>
        <skos:definition xml:lang="en">An Actuation carries out an (Actuation) Procedure to change the state of the world using an Actuator.</skos:definition>
        <skos:example xml:lang="en">The activity of automatically closing a window if the temperature in a room drops below 20 degree Celsius. The activity is the Actuation and the device that closes the window is the Actuator. The Procedure is the rule, plan, or specification that defines the conditions that triggers the Actuation, here a drop in temperature. </skos:example>
    </owl:Class>

    <!-- http://www.w3.org/ns/sosa/Actuator -->

    <owl:Class rdf:about="http://www.w3.org/ns/sosa/Actuator">
        <rdfs:subClassOf rdf:resource="http://www.w3.org/ns/ssn/System"/>
        <rdfs:subClassOf>
            <owl:Restriction>
                <owl:onProperty rdf:resource="http://www.w3.org/ns/sosa/madeActuation"/>
                <owl:allValuesFrom rdf:resource="http://www.w3.org/ns/sosa/Actuation"/>
            </owl:Restriction>
        </rdfs:subClassOf>
        <rdfs:subClassOf>
            <owl:Restriction>
                <owl:onProperty rdf:resource="http://www.w3.org/ns/ssn/forProperty"/>
                <owl:allValuesFrom rdf:resource="http://www.w3.org/ns/sosa/ActuatableProperty"/>
            </owl:Restriction>
        </rdfs:subClassOf>
        <owl:disjointWith rdf:resource="http://www.w3.org/ns/sosa/Sensor"/>
        <rdfs:comment xml:lang="en">A device that is used by, or implements, an (Actuation) Procedure that changes the state of the world.</rdfs:comment>
        <rdfs:isDefinedBy rdf:resource="http://www.w3.org/ns/sosa/"/>
        <rdfs:label xml:lang="en">Actuator</rdfs:label>
        <skos:definition xml:lang="en">A device that is used by, or implements, an (Actuation) Procedure that changes the state of the world.</skos:definition>
        <skos:example xml:lang="en">A window actuators for automatic window control, i.e., opening or closing the window.</skos:example>
    </owl:Class>

    <!-- http://www.w3.org/ns/sosa/FeatureOfInterest -->

    <owl:Class rdf:about="http://www.w3.org/ns/sosa/FeatureOfInterest">
        <rdfs:subClassOf>
            <owl:Restriction>
                <owl:onProperty rdf:resource="http://www.w3.org/ns/ssn/hasProperty"/>
                <owl:allValuesFrom rdf:resource="http://www.w3.org/ns/ssn/Property"/>
            </owl:Restriction>
        </rdfs:subClassOf>
        <rdfs:subClassOf>
            <owl:Restriction>
                <owl:onProperty rdf:resource="http://www.w3.org/ns/ssn/hasProperty"/>
                <owl:minCardinality rdf:datatype="http://www.w3.org/2001/XMLSchema#nonNegativeInteger">1</owl:minCardinality>
            </owl:Restriction>
        </rdfs:subClassOf>
        <rdfs:comment xml:lang="en">The thing whose property is being estimated or calculated in the course of an Observation to arrive at a Result or whose property is being manipulated by an Actuator, or which is being sampled or transformed in an act of Sampling.</rdfs:comment>
        <rdfs:isDefinedBy rdf:resource="http://www.w3.org/ns/sosa/"/>
        <rdfs:label xml:lang="en">Feature Of Interest</rdfs:label>
        <skos:definition xml:lang="en">The thing whose property is being estimated or calculated in the course of an Observation to arrive at a Result or whose property is being manipulated by an Actuator, or which is being sampled or transformed in an act of Sampling.</skos:definition>
        <skos:example xml:lang="en">When measuring the height of a tree, the height is the observed ObservableProperty, 20m may be the Result of the Observation, and the tree is the FeatureOfInterest. A window is a FeatureOfInterest for an automatic window control Actuator.</skos:example>
    </owl:Class>

    <!-- http://www.w3.org/ns/sosa/ObservableProperty -->

    <owl:Class rdf:about="http://www.w3.org/ns/sosa/ObservableProperty">
        <rdfs:subClassOf rdf:resource="http://www.w3.org/ns/ssn/Property"/>
        <rdfs:subClassOf>
            <owl:Restriction>
                <owl:onProperty rdf:resource="http://www.w3.org/ns/sosa/isObservedBy"/>
                <owl:allValuesFrom rdf:resource="http://www.w3.org/ns/sosa/Sensor"/>
            </owl:Restriction>
        </rdfs:subClassOf>
        <rdfs:subClassOf>
            <owl:Restriction>
                <owl:onProperty>
                    <rdf:Description>
                        <owl:inverseOf rdf:resource="http://www.w3.org/ns/sosa/observedProperty"/>
                    </rdf:Description>
                </owl:onProperty>
                <owl:allValuesFrom rdf:resource="http://www.w3.org/ns/sosa/Observation"/>
            </owl:Restriction>
        </rdfs:subClassOf>
        <rdfs:comment xml:lang="en">An observable quality (property, characteristic) of a FeatureOfInterest.</rdfs:comment>
        <rdfs:isDefinedBy rdf:resource="http://www.w3.org/ns/sosa/"/>
        <rdfs:label xml:lang="en">Observable Property</rdfs:label>
        <skos:definition xml:lang="en">An observable quality (property, characteristic) of a FeatureOfInterest.</skos:definition>
        <skos:example xml:lang="en">The height of a tree, the depth of a water body, or the temperature of a surface are examples of observable properties, while the value of a classic car is not (directly) observable but asserted.</skos:example>
    </owl:Class>

    <!-- http://www.w3.org/ns/sosa/Observation -->

    <owl:Class rdf:about="http://www.w3.org/ns/sosa/Observation">
        <rdfs:subClassOf>
            <owl:Restriction>
                <owl:onProperty rdf:resource="http://www.w3.org/ns/sosa/hasFeatureOfInterest"/>
                <owl:allValuesFrom rdf:resource="http://www.w3.org/ns/sosa/FeatureOfInterest"/>
            </owl:Restriction>
        </rdfs:subClassOf>
        <rdfs:subClassOf>
            <owl:Restriction>
                <owl:onProperty rdf:resource="http://www.w3.org/ns/sosa/madeBySensor"/>
                <owl:allValuesFrom rdf:resource="http://www.w3.org/ns/sosa/Sensor"/>
            </owl:Restriction>
        </rdfs:subClassOf>
        <rdfs:subClassOf>
            <owl:Restriction>
                <owl:onProperty rdf:resource="http://www.w3.org/ns/sosa/observedProperty"/>
                <owl:allValuesFrom rdf:resource="http://www.w3.org/ns/sosa/ObservableProperty"/>
            </owl:Restriction>
        </rdfs:subClassOf>
        <rdfs:subClassOf>
            <owl:Restriction>
                <owl:onProperty rdf:resource="http://www.w3.org/ns/sosa/hasFeatureOfInterest"/>
                <owl:cardinality rdf:datatype="http://www.w3.org/2001/XMLSchema#nonNegativeInteger">1</owl:cardinality>
            </owl:Restriction>
        </rdfs:subClassOf>
        <rdfs:subClassOf>
            <owl:Restriction>
                <owl:onProperty rdf:resource="http://www.w3.org/ns/sosa/madeBySensor"/>
                <owl:cardinality rdf:datatype="http://www.w3.org/2001/XMLSchema#nonNegativeInteger">1</owl:cardinality>
            </owl:Restriction>
        </rdfs:subClassOf>
        <rdfs:subClassOf>
            <owl:Restriction>
                <owl:onProperty rdf:resource="http://www.w3.org/ns/sosa/observedProperty"/>
                <owl:cardinality rdf:datatype="http://www.w3.org/2001/XMLSchema#nonNegativeInteger">1</owl:cardinality>
            </owl:Restriction>
        </rdfs:subClassOf>
        <rdfs:subClassOf>
            <owl:Restriction>
                <owl:onProperty rdf:resource="http://www.w3.org/ns/sosa/resultTime"/>
                <owl:cardinality rdf:datatype="http://www.w3.org/2001/XMLSchema#nonNegativeInteger">1</owl:cardinality>
            </owl:Restriction>
        </rdfs:subClassOf>
        <rdfs:comment xml:lang="en">Act of carrying out an (Observation) Procedure to estimate or calculate a value of a property of a FeatureOfInterest. Links to a Sensor to describe what made the Observation and how; links to an ObservableProperty to describe what the result is an estimate of, and to a FeatureOfInterest to detail what that property was associated with.</rdfs:comment>
        <rdfs:isDefinedBy rdf:resource="http://www.w3.org/ns/sosa/"/>
        <rdfs:label xml:lang="en">Observation</rdfs:label>
        <skos:definition xml:lang="en">Act of carrying out an (Observation) Procedure to estimate or calculate a value of a property of a FeatureOfInterest. Links to a Sensor to describe what made the Observation and how; links to an ObservableProperty to describe what the result is an estimate of, and to a FeatureOfInterest to detail what that property was associated with.</skos:definition>
        <skos:example xml:lang="en">The activity of estimating the intensity of an Earthquake using the Mercalli intensity scale is an Observation as is measuring the moment magnitude, i.e., the energy released by said earthquake.</skos:example>
    </owl:Class>

    <!-- http://www.w3.org/ns/sosa/Platform -->

    <owl:Class rdf:about="http://www.w3.org/ns/sosa/Platform">
        <rdfs:subClassOf>
            <owl:Restriction>
                <owl:onProperty rdf:resource="http://www.w3.org/ns/sosa/hosts"/>
                <owl:someValuesFrom rdf:resource="http://www.w3.org/ns/sosa/FeatureOfInterest"/>
            </owl:Restriction>
        </rdfs:subClassOf>
        <rdfs:subClassOf>
            <owl:Restriction>
                <owl:onProperty rdf:resource="http://www.w3.org/ns/sosa/hosts"/>
                <owl:someValuesFrom rdf:resource="http://www.w3.org/ns/ssn/System"/>
            </owl:Restriction>
        </rdfs:subClassOf>
        <rdfs:subClassOf>
            <owl:Restriction>
                <owl:onProperty rdf:resource="http://www.semanticweb.org/decentralized-context-aware-ontology#has_location"/>
                <owl:allValuesFrom rdf:resource="http://www.semanticweb.org/decentralized-context-aware-ontology#Location"/>
            </owl:Restriction>
        </rdfs:subClassOf>
        <rdfs:comment xml:lang="en">A Platform is an entity that hosts other entities, particularly Sensors, Actuators, Samplers, and other Platforms.</rdfs:comment>
        <rdfs:isDefinedBy rdf:resource="http://www.w3.org/ns/sosa/"/>
        <rdfs:label xml:lang="en">Platform</rdfs:label>
        <skos:definition xml:lang="en">A Platform is an entity that hosts other entities, particularly Sensors, Actuators, Samplers, and other Platforms.</skos:definition>
        <skos:example xml:lang="en">A post, buoy, vehicle, ship, aircraft, satellite, cell-phone, human or animal may act as platforms for (technical or biological) sensors or actuators.</skos:example>
    </owl:Class>

    <!-- http://www.w3.org/ns/sosa/Result -->

    <owl:Class rdf:about="http://www.w3.org/ns/sosa/Result">
        <rdfs:comment xml:lang="en">The Result of an Observation, Actuation, or act of Sampling. To store an observation&apos;s simple result value one can use the hasSimpleResult property.</rdfs:comment>
        <rdfs:isDefinedBy rdf:resource="http://www.w3.org/ns/sosa/"/>
        <rdfs:label xml:lang="en">Result</rdfs:label>
        <skos:definition xml:lang="en">The Result of an Observation, Actuation, or act of Sampling. To store an observation&apos;s simple result value one can use the hasSimpleResult property.</skos:definition>
        <skos:example xml:lang="en">The value 20 as the height of a certain tree together with the unit, e.g., Meter.</skos:example>
    </owl:Class>

    <!-- http://www.w3.org/ns/sosa/Sensor -->

    <owl:Class rdf:about="http://www.w3.org/ns/sosa/Sensor">
        <rdfs:subClassOf rdf:resource="http://www.w3.org/ns/ssn/System"/>
        <rdfs:subClassOf>
            <owl:Restriction>
                <owl:onProperty rdf:resource="http://www.w3.org/ns/sosa/madeObservation"/>
                <owl:allValuesFrom rdf:resource="http://www.w3.org/ns/sosa/Observation"/>
            </owl:Restriction>
        </rdfs:subClassOf>
        <rdfs:subClassOf>
            <owl:Restriction>
                <owl:onProperty rdf:resource="http://www.w3.org/ns/sosa/observes"/>
                <owl:allValuesFrom rdf:resource="http://www.w3.org/ns/sosa/ObservableProperty"/>
            </owl:Restriction>
        </rdfs:subClassOf>
        <rdfs:comment xml:lang="en">Device, agent (including humans), or software (simulation) involved in, or implementing, a Procedure. Sensors respond to a stimulus, e.g., a change in the mode, or input data composed from the results of prior Observations, and generate a Result. Sensors can be hosted by Platforms.</rdfs:comment>
        <rdfs:isDefinedBy rdf:resource="http://www.w3.org/ns/sosa/"/>
        <rdfs:label xml:lang="en">Sensor</rdfs:label>
        <skos:definition xml:lang="en">Device, agent (including humans), or software (simulation) involved in, or implementing, a Procedure. Sensors respond to a stimulus, e.g., a change in the mode, or input data composed from the results of prior Observations, and generate a Result. Sensors can be hosted by Platforms.</skos:definition>
        <skos:example xml:lang="en">Accelerometers, gyroscopes, barometers, magnetometers, and so forth are Sensors that are typically mounted on a modern smart phone (which acts as Platform). Other examples of sensors include the human eyes.</skos:example>
    </owl:Class>

    <!-- http://www.w3.org/ns/ssn/Property -->

    <owl:Class rdf:about="http://www.w3.org/ns/ssn/Property">
        <rdfs:subClassOf>
            <owl:Restriction>
                <owl:onProperty rdf:resource="http://www.w3.org/ns/ssn/isPropertyOf"/>
                <owl:allValuesFrom rdf:resource="http://www.w3.org/ns/sosa/FeatureOfInterest"/>
            </owl:Restriction>
        </rdfs:subClassOf>
        <rdfs:comment xml:lang="en">A quality of an entity. An aspect of an entity that is intrinsic to and cannot exist without the entity.</rdfs:comment>
        <rdfs:isDefinedBy rdf:resource="http://www.w3.org/ns/ssn/"/>
        <rdfs:label xml:lang="en">Property</rdfs:label>
        <skos:definition xml:lang="en">A quality of an entity. An aspect of an entity that is intrinsic to and cannot exist without the entity.</skos:definition>
    </owl:Class>

    <!-- http://www.w3.org/ns/ssn/System -->

    <owl:Class rdf:about="http://www.w3.org/ns/ssn/System">
        <rdfs:subClassOf>
            <owl:Restriction>
                <owl:onProperty rdf:resource="http://www.semanticweb.org/decentralized-context-aware-ontology#has_location"/>
                <owl:allValuesFrom rdf:resource="http://www.semanticweb.org/decentralized-context-aware-ontology#Location"/>
            </owl:Restriction>
        </rdfs:subClassOf>
        <rdfs:subClassOf>
            <owl:Restriction>
                <owl:onProperty rdf:resource="http://www.w3.org/ns/sosa/isHostedBy"/>
                <owl:allValuesFrom rdf:resource="http://www.w3.org/ns/sosa/Platform"/>
            </owl:Restriction>
        </rdfs:subClassOf>
        <rdfs:comment xml:lang="en">System is a unit of abstraction for pieces of infrastructure that implement Procedures. A System may have components, its subsystems, which are other systems.</rdfs:comment>
        <rdfs:isDefinedBy rdf:resource="http://www.w3.org/ns/ssn/"/>
        <rdfs:label xml:lang="en">System</rdfs:label>
        <skos:definition xml:lang="en">System is a unit of abstraction for pieces of infrastructure that implement Procedures. A System may have components, its subsystems, which are other systems.</skos:definition>
    </owl:Class>

    <!-- 
    ///////////////////////////////////////////////////////////////////////////////////////
    //
    // Individuals
    //
    ///////////////////////////////////////////////////////////////////////////////////////
     -->

     <!-- http://www.semanticweb.org/decentralized-context-aware-ontology#855a01f8-8e8c-4561-be83-eee2d967555d -->

      <owl:NamedIndividual rdf:about="http://www.semanticweb.org/decentralized-context-aware-ontology#855a01f8-8e8c-4561-be83-eee2d967555d">
          <rdf:type rdf:resource="http://www.semanticweb.org/decentralized-context-aware-ontology#Processing_Material"/>
          <decas:min_temperature rdf:datatype="http://www.w3.org/2001/XMLSchema#decimal">18</decas:min_temperature>
          <decas:max_temperature rdf:datatype="http://www.w3.org/2001/XMLSchema#decimal">20</decas:max_temperature>
          <rdfs:comment xml:lang="en">A liquid that is mixed during the mixing process. It is a compound of water and hot water.</rdfs:comment>
          <rdfs:label xml:lang="en">Mixing Water</rdfs:label>
          <skos:definition xml:lang="en">A liquid that is mixed during the mixing process. It is a compound of water and hot water.</skos:definition>
      </owl:NamedIndividual>

    <!-- http://www.semanticweb.org/decentralized-context-aware-ontology#a48538a8-76a6-48ca-ae66-7620957fb9a6 -->

    <owl:NamedIndividual rdf:about="http://www.semanticweb.org/decentralized-context-aware-ontology#a48538a8-76a6-48ca-ae66-7620957fb9a6">
        <rdf:type rdf:resource="http://www.semanticweb.org/decentralized-context-aware-ontology#Switch_Actuator"/>
        <decas:has_location rdf:resource="http://www.semanticweb.org/decentralized-context-aware-ontology#eedf88d1-db25-4847-bc00-4571a8eb65d9"/>
        <sosa:isHostedBy rdf:resource="http://www.semanticweb.org/decentralized-context-aware-ontology#81b39cd2-721d-4452-91f2-325eea8e5666"/>
        <decas:is_established rdf:datatype="http://www.w3.org/2001/XMLSchema#boolean">true</decas:is_established>
<!--         <sosa:madeActuation rdf:resource="http://www.semanticweb.org/decentralized-context-aware-ontology#607f503c-29d4-4c05-bd2d-eb82defb9d71"/> -->
        <rdfs:comment xml:lang="en">An electric switch actuators to activate or deactivate the agitator device.</rdfs:comment>
        <rdfs:label xml:lang="en">Mixer Agitator Switch</rdfs:label>
        <skos:definition xml:lang="en">An electric switch actuators to activate or deactivate the agitator device.</skos:definition>
    </owl:NamedIndividual>

    <!-- http://www.semanticweb.org/decentralized-context-aware-ontology#d29db2d2-8fe3-4ae0-9186-8b38929f7cfd -->

    <owl:NamedIndividual rdf:about="http://www.semanticweb.org/decentralized-context-aware-ontology#d29db2d2-8fe3-4ae0-9186-8b38929f7cfd">
        <rdf:type rdf:resource="http://www.semanticweb.org/decentralized-context-aware-ontology#Agitator"/>
        <rdfs:comment xml:lang="en">A device to mix the materials within a material container.</rdfs:comment>
        <rdfs:label xml:lang="en">Mixer Agitator</rdfs:label>
        <skos:definition xml:lang="en">A device to mix the materials within a material container.</skos:definition>
    </owl:NamedIndividual>

    <!-- http://www.semanticweb.org/decentralized-context-aware-ontology#eedf88d1-db25-4847-bc00-4571a8eb65d9 -->

    <owl:NamedIndividual rdf:about="http://www.semanticweb.org/decentralized-context-aware-ontology#eedf88d1-db25-4847-bc00-4571a8eb65d9">
        <rdf:type rdf:resource="http://www.semanticweb.org/decentralized-context-aware-ontology#Location"/>
        <decas:is_location_of rdf:resource="http://www.semanticweb.org/decentralized-context-aware-ontology#81b39cd2-721d-4452-91f2-325eea8e5666"/>
        <rdfs:comment xml:lang="en">A Flash Mixing salon is a location where the flash mixer equipment is kept.</rdfs:comment>
        <rdfs:label xml:lang="en">Flash Mixing Salon</rdfs:label>
        <skos:definition xml:lang="en">A Flash Mixing salon is a location where the flash mixer equipment is kept.</skos:definition>
    </owl:NamedIndividual>

    <!-- http://www.semanticweb.org/decentralized-context-aware-ontology#057a35eb-8b62-41c8-9806-44f071cfad03 -->

    <owl:NamedIndividual rdf:about="http://www.semanticweb.org/decentralized-context-aware-ontology#057a35eb-8b62-41c8-9806-44f071cfad03">
        <rdf:type rdf:resource="http://www.semanticweb.org/decentralized-context-aware-ontology#Temperature_Sensor"/>
        <decas:has_location rdf:resource="http://www.semanticweb.org/decentralized-context-aware-ontology#eedf88d1-db25-4847-bc00-4571a8eb65d9"/>
        <sosa:observes rdf:resource="http://www.semanticweb.org/decentralized-context-aware-ontology#855a01f8-8e8c-4561-be83-eee2d967555d"/>
        <sosa:isHostedBy rdf:resource="http://www.semanticweb.org/decentralized-context-aware-ontology#81b39cd2-721d-4452-91f2-325eea8e5666"/>
        <decas:is_established rdf:datatype="http://www.w3.org/2001/XMLSchema#boolean">true</decas:is_established>
        <rdfs:comment xml:lang="en">A temperature sensor in the mixing material container monitors the temperature of the processing material with the technical code of DS18B20.</rdfs:comment>
        <rdfs:label xml:lang="en">Mixer Temperature Sensor</rdfs:label>
        <skos:definition xml:lang="en">A temperature sensor in the mixing material container monitors the temperature of the processing material with the technical code of DS18B20.</skos:definition>
    </owl:NamedIndividual>

<!--      --><!--  --><!-- http://www.semanticweb.org/decentralized-context-aware-ontology#607f503c-29d4-4c05-bd2d-eb82defb9d71 -->

<!--     <owl:NamedIndividual rdf:about="http://www.semanticweb.org/decentralized-context-aware-ontology#607f503c-29d4-4c05-bd2d-eb82defb9d71"> -->
<!--         <rdf:type rdf:resource="http://www.semanticweb.org/decentralized-context-aware-ontology#Mixer_Agitator_Actuation"/> -->
<!--         <sosa:hasFeatureOfInterest rdf:resource="http://www.semanticweb.org/decentralized-context-aware-ontology#d29db2d2-8fe3-4ae0-9186-8b38929f7cfd"/> -->
<!--         <sosa:madeByActuator rdf:resource="http://www.semanticweb.org/decentralized-context-aware-ontology#a48538a8-76a6-48ca-ae66-7620957fb9a6"/> -->
<!--         <decas:is_active rdf:datatype="http://www.w3.org/2001/XMLSchema#boolean">true</decas:is_active> -->
<!--         <rdfs:comment xml:lang="en">Actuation state relating to the agitator of the flash mixer machine.</rdfs:comment> -->
<!--         <rdfs:label xml:lang="en">Mixer Agitator Actuation</rdfs:label> -->
<!--         <skos:definition xml:lang="en">Actuation state relating to the agitator of the flash mixer machine.</skos:definition> -->
<!--     </owl:NamedIndividual> -->

    <!-- http://www.semanticweb.org/decentralized-context-aware-ontology#81b39cd2-721d-4452-91f2-325eea8e5666 -->

    <owl:NamedIndividual rdf:about="http://www.semanticweb.org/decentralized-context-aware-ontology#81b39cd2-721d-4452-91f2-325eea8e5666">
        <rdf:type rdf:resource="http://www.semanticweb.org/decentralized-context-aware-ontology#Flash_Mixer_Machine"/>
        <decas:has_location rdf:resource="http://www.semanticweb.org/decentralized-context-aware-ontology#eedf88d1-db25-4847-bc00-4571a8eb65d9"/>
        <sosa:hosts rdf:resource="http://www.semanticweb.org/decentralized-context-aware-ontology#a48538a8-76a6-48ca-ae66-7620957fb9a6"/>
        <sosa:hosts rdf:resource="http://www.semanticweb.org/decentralized-context-aware-ontology#057a35eb-8b62-41c8-9806-44f071cfad03"/>
        <decas:is_active rdf:datatype="http://www.w3.org/2001/XMLSchema#boolean">false</decas:is_active>
        <rdfs:comment xml:lang="en">An equipment disperses and mixes raw materials into the production process stream.</rdfs:comment>
        <rdfs:label xml:lang="en">Flash Mixer Machine</rdfs:label>
        <skos:definition xml:lang="en">An equipment disperses and mixes raw materials into the production process stream.</skos:definition>
    </owl:NamedIndividual>

</rdf:RDF>



<!-- Generated by the OWL API (version 4.5.25.2023-02-15T19:15:49Z) https://github.com/owlcs/owlapi -->

